# Problem Explanation

This problem is kind of hard, so does the implementation

In linked list problem, <br>
***Always compare the input and output***<br>
***See how to re-wire the node to solve the problem***<br>

Note that both solution need some complex re-wiring<br>

## First Solution
I came up with this solution by myself<br>
But the time complexity is bad<br>

Let's see the example<br>
input:  [1,2,3,4,5]<br>
output: [1,5,2,4,3]<br>

It seems that the first node has to connect to the last node<br>
And last node connects to the second node<br>
f = first node<br>
l = last node<br>
<pre>
f                   l
1    2 -> 3 -> 4 -> 5
  \ /
   5
   l
</pre>
And now we have to update the first node to `2`
And update the last node to `4`<br>

We seems to have a pattern here<br>
1. First node connects to the last node
2. Last node connects to the second node
3. Update first node to the second node
4. Update last node to the second last node

This is just the high level idea<br>
We have two details to note<br>
1. We somehow have to set the next of node before tail to `nullptr`
  - In the above example, we have to manually set `4->next` to `nullptr`
  - So that `4` becomes real tail
2. We have to reference the next node before we update the node
  - In the above example, we have to reference `2` before we update `1` to `5`
  - Without this, we will lose the reference to `2` after re-wiring

Finally, let's see one edge case<br>
1. Two nodes
<pre>
f    l
1 -> 2
</pre>
`curNextNode` is `2`<br>
`tail` is also `2`<br>
We know we have to stop here<br>

Let's see all the steps<br>
1. Find the tail, and the node before tail
2. Reference the current next node
3. Check if `curNextNode` is `tail`
4. Set `ptr->next` to `tail`
5. Set `tail->next` to `curNextNode`
6. Set `nodeBeforeTail->next` to `nullptr`
7. Update `ptr` to `curNextNode`

Input:  [1,2,3,4,5]<br>
p = ptr<br>
l = tail<br>
bl = nodeBeforeTail<br>
n = curNextNode<br>
1. Find the tail, and the node before tail
<pre>
p              bl   l
1 -> 2 -> 3 -> 4 -> 5
</pre>

2. Reference the current next node
<pre>
p    n         bl   l
1 -> 2 -> 3 -> 4 -> 5
</pre>

3. Check if `curNextNode` is `tail`
4. Set `ptr->next` to `tail`
<pre>
p    n         bl   l
1   2 -> 3 -> 4 -> 5
 \ --------------- /
</pre>

5. Set `tail->next` to `curNextNode`
<pre>
p    n         bl   l
1   2 -> 3 -> 4 -> 5
 \  /
  5
</pre>

6. Set `nodeBeforeTail->next` to `nullptr`
<pre>
p    n        bl  
1   2 -> 3 -> 4 -> x
 \  /
  5
</pre>

7. Update `ptr` to `curNextNode`
<pre>
    p
1   2 -> 3 -> 4 -> x
 \  /
  5
</pre>

Again!!<br>

1. Find the tail, and the node before tail
<pre>
          p   bl    l
1 -> 5 -> 2 -> 3 -> 4 -> x
</pre>

2. Reference the current next node
<pre>
               n   
          p    bl   l
1 -> 5 -> 2 -> 3 -> 4 -> x
</pre>

3. Check if `curNextNode` is `tail`
4. Set `ptr->next` to `tail`
<pre>
               bl   
          p    n    l
1 -> 5 -> 2   3 -> 4 -> x
          \ ------- /
</pre>

5. Set `tail->next` to `curNextNode`
<pre>
               bl   
          p    n    l
1 -> 5 -> 2   3 -> 4 -> x
          \    /
            4 
</pre>

6. Set `nodeBeforeTail->next` to `nullptr`
<pre>
               bl   
          p    n    
1 -> 5 -> 2   3 -> x
          \    /
            4 
</pre>

7. Update `ptr` to `curNextNode`
<pre>
                    p
1 -> 5 -> 2 -> 4 -> 3 -> x
</pre>
Done!!

### Complexity Analysis

#### Time Complexity: O(n ^ 2)
- We have to find the tail and the node before tail
  - So there's a nested loop

#### Space Complexity: O(1)

## Second Solution
This solution is kind of tricky<br>
Let's look at the example<br>
input:  [1,2,3,4,5]<br>
output: [1,5,2,4,3]<br>

If we cut the list in the middle, we have two lists<br>
1. [1,2,3]<br>
2. [4,5]<br>

We reverse the second list<br>
1. [1,2,3]<br>
2. [5,4]<br>

And then we merge the two lists<br>
[1,5,2,4,3]<br>
This is the answer<br>

So the high level idea is<br>
1. Find the middle of the list
2. Reverse the second list
3. Merge the two lists

Let's walk through the example<br>
input:  [1,2,3,4,5]<br>
1. Find the middle of the list
<pre>
          s
                    f
1 -> 2 -> 3 -> 4 -> 5
</pre>
`s` is at the middle<br>
Now, we have two lists<br>
[1,2,3]<br>
[4,5] (s->next is the second list)<br>

2. Reverse the second list
<pre>
          s
1 -> 2 -> 3 -> 4 

p      
5 -> 4 -> x 
</pre>
`p` is the previous node after reversing<br>
At this point, `s->next` still points to `4`<br>
So we have to set `s->next` to `nullptr`<br>

3. Merge the two lists<br>
f = firstList<br>
s = secondList<br>
fn = firstNext<br>
sn = secondNext<br>

(1) reference the next node<br>
<pre>
f   fn
1 -> 2 -> 3 -> x
5 -> 4 -> x
s    sn
</pre>

(2) re-wire the node<br>
`f->next = s`<br>
`s->next = fn`<br>
<pre>
f   fn
1   2 -> 3 -> x
|  /
5 / 4 -> x
s   sn
</pre>

(3) update the pointer<br>
<pre>
    f
1   2 -> 3 -> x
|  /
5 / 4 -> x
    s
</pre>

(1) reference the next node<br>
<pre>
    f   fn
1   2 -> 3 -> x
|  /
5 / 4 -> x
    s   sn
</pre>
  
(2) re-wire the node<br>
`fn->next = s`<br>
`s->next = fn`<br>
<pre>
    f   fn
1   2    3 -> x
|  /  |  /
5 /   4 / x
      s    sn
</pre>

We are done<br>
<pre>
1 -> 5 -> 2 -> 4 -> 3 -> x
</pre>

### Complexity Analysis

#### Time Complexity: O(n)
#### Space Complexity: O(1)

## Third Solution
The idea of this solution is not that hard.<br>
We just use an array to store all the nodes in order<br>
Then we use two pointers technique to re-wire the nodes<br>

However, there's a lot of edge cases to consider<br>
1. Have to break the link of each node when adding to the array
   - Each element in the array should be a node without any dependency(next pointer)
   - It's easier to re-wire the nodes in the next step
2. How to handle the re-wiring?
   - Odd Case
     - [1,2,3,4,5], correct answer is [1,5,2,4,3]
     - when left = 2, right = 4
      - make 2 -> 4
      - left++
      - left != right
      - make 4 -> 3
      - right--
    - When consider the condition again, left = 3, right = 3, break the loop
   - Even Case
     - [1,2,3,4]
     - when left = 2, right = 3
      - make 2 -> 3
      - left++
      - left == right, break the loop
   - So, after incrementing the left pointer, we have to check if it equals to the right pointer
     - If yes, break the loop
     - If no, make the right pointer's next point to the left pointer
